msl/shares.v
@@ -297,15 +297,26 @@ Proof.
   rewrite lub_bot in H0. apply nontrivial; auto.
 Qed.  
 
-Lemma bot_joins : forall x, joins bot x.
+Lemma bot_join_eq : forall x, join bot x x.
 Proof.
-  intro x; exists x.
+  intros.
   destruct (join_ex_identities x); intuition.
   destruct H0.
   generalize (H _ _ H0).
   intros; subst; auto.
   replace bot with x0; auto.
   apply identity_share_bot; auto.
+Qed.
+
+Lemma join_bot_eq : forall x, join x bot x.
+Proof.
+  intros.
+  apply join_comm, bot_join_eq.
+Qed.
+
+Lemma bot_joins : forall x, joins bot x.
+Proof.
+  intro x; exists x; apply bot_join_eq.
 Qed.
 
 Lemma dec_share_identity : forall x:t, { identity x } + { ~identity x }.
